status.sh
@@ -1,0 +1,3 @@
+#!/usr/bin/env bash
+
+egrep -i "(admit|todo)" src/*/*.v
